Knorm.v
@@ -1,0 +1,277 @@
+Require Import Omega.
+
+Require Import Continuation.
+Require Import Rewrites.
+Require Import Norm.
+Require Import Term.
+
+(** * More Induction Principles on Reduction Sequences *)
+(** These require knowledge of Continuation.v, so can't be placed in Norm.v *)
+(** Continuations have their own "strong normalization" on their own reduction
+    rule. *)
+Inductive Krw_norm K :=
+  reducts_Krw_norm : (forall K', Krw K K' -> Krw_norm K') -> Krw_norm K.
+
+Inductive Triple_SN K M N :=
+  | triple_sn :
+       (forall K', (Krw K K') -> Triple_SN K' M N)
+    -> (forall M', (M ~> M') -> Triple_SN K M' N)
+    -> (forall N', (N ~> N') -> Triple_SN K M N')
+    -> Triple_SN K M N.
+
+Lemma triple_induction_via_TripleSN P:
+  (forall K M N,
+        (forall K',  (Krw K K') -> P K' M N)
+     -> (forall M',  (M ~> M') ->  P K M' N)
+     -> ((forall N', (N ~> N') ->  P K M N'))
+     -> P K M N)
+  ->
+  forall K M N,
+    Triple_SN K M N -> P K M N.
+Proof.
+ intros IH K M N SN_K_M_N.
+ induction SN_K_M_N.
+ auto.
+Qed.
+
+Lemma triple_induction_via_TripleSN_scoped P:
+  forall K0 M0 N0,
+  (forall K M N,
+     Krw_rt K0 K -> (M0 ~>> M) -> (N0 ~>> N) ->
+        (forall K',  (Krw K K') -> P K' M N)
+     -> (forall M',  (M ~> M') ->  P K M' N)
+     -> ((forall N', (N ~> N') ->  P K M N'))
+     -> P K M N)
+  ->
+    Triple_SN K0 M0 N0 -> P K0 M0 N0.
+Proof.
+ intros K0 M0 N0 IH SN_K0_M0_N0.
+ induction SN_K0_M0_N0.
+ apply IH; auto.
+ intros; apply X; auto.
+ intros; apply IH; eauto.
+ intros; apply X0; auto.
+ intros; apply IH; eauto.
+ intros; apply X1; auto.
+ intros; apply IH; eauto.
+Qed.
+
+Lemma Triple_SN_intro:
+  forall K, Krw_norm K -> forall M, SN M -> forall N, SN N -> Triple_SN K M N.
+Proof.
+ intros K SN_K.
+ induction SN_K.
+ intros M SN_M.
+ induction SN_M.
+ intros N SN_N.
+ induction SN_N.
+ constructor; sauto.
+Qed.
+
+Lemma triple_induction_scoped P:
+  forall K0 M0 N0,
+  (forall K M N,
+     Krw_rt K0 K -> (M0 ~>> M) -> (N0 ~>> N) ->
+        (forall K',  (Krw K K') -> P K' M N)
+     -> (forall M',  (M ~> M') ->  P K M' N)
+     -> ((forall N', (N ~> N') ->  P K M N'))
+     -> P K M N)
+  ->
+    Krw_norm K0 -> SN M0 -> SN N0 -> P K0 M0 N0.
+Proof.
+ intros K0 M0 N0 IH SN_K0 SN_M0 SN_N0.
+ apply triple_induction_via_TripleSN_scoped; auto.
+ apply Triple_SN_intro; auto.
+Qed.
+
+(** A continuation that is part of, and downstream of, a SN term, is normalizing. *)
+Lemma SN_context_Krw_norm:
+  forall X X',
+    SN X ->
+    (X ~>> X') ->
+    forall K,
+    {M : Term & X' = plug K M} ->
+    Krw_norm K.
+Proof.
+ intros X X' SN_X X_red_X'.
+ assert (SN_X' : SN X').
+  eauto.
+ induction SN_X'.
+ intros K ex_M.
+ constructor.
+ intros K' K_K'.
+ destruct ex_M as [M H1].
+ assert (plug K M ~> plug K' M) by auto.
+ subst.
+ apply H with (m':=plug K' M); eauto.
+Qed.
+
+Lemma SN_via_Krw_rt :
+  forall K K' M,
+    Krw_rt K K' -> SN (plug K M) -> SN (plug K' M).
+Proof.
+ intros.
+ assert (plug K M ~>> plug K' M).
+  auto using Krw_rt_Rw_rt.
+ eauto using Rw_trans_preserves_SN.
+Qed.
+
+Lemma SN_via_Krw :
+  forall K K' M,
+    Krw K K' -> SN (plug K M) -> SN (plug K' M).
+Proof.
+ intros.
+ assert (plug K M ~> plug K' M).
+  auto.
+ eauto using Rw_trans_preserves_SN.
+Qed.
+
+Lemma Krw_norm_from_SN:
+  forall Q, SN Q -> forall K M, (Q ~>> plug K M) -> Krw_norm K.
+Proof.
+ intros Q H.
+ induction H.
+ constructor.
+ intros.
+ eapply last_step_first_step_lemma in H0.
+  destruct H0.
+  destruct p.
+  eapply H; eauto.
+ eauto.
+Qed.
+
+Lemma SN_K_M_SN_K_Null:
+  forall K M,
+    SN (plug K M) ->
+    SN (plug K TmNull).
+Proof.
+ induction K using Ksize_induction_strong.
+ rename H into IHK.
+ intros M H0.
+ apply SN_embedding2 with
+     (f := fun k => plug k M)
+     (g := fun k => plug k TmNull)
+     (Q := plug K M)
+     (Q' := plug K TmNull); try auto.
+ intros K0 Z H2 H3.
+
+ let T := type of H3 in copy T.
+ apply K_TmNull_rw in H3 as [[K_shorter [N H1a H1b]] | [K' H1a H1b]].
+ (* Case [plug K0 TmNull] drops a frame. *)
+  right.
+  subst.
+
+  (* XXX this is terribly ugly. must be a simpler way *)
+  assert (relK_rt K K_shorter).
+   assert (relK_rt K (Iterate N K_shorter)).
+    apply K_TmNull_relK_rt.
+    auto.
+   apply trans with (K' := Iterate N K_shorter).
+    auto.
+   apply step.
+   eapply strip; eauto.
+  apply magic with (M:=M) in H1; auto.
+
+  destruct H1 as [M' SN_M'].
+
+  apply IHK with (M:=M'); auto.
+  apply Rw_rt_conserves_Ksize in H2.
+  simpl in *; sauto.
+
+ (* Case K0 ~> K' *)
+ left.
+ exists K'.
+ firstorder.
+Qed.
+
+Lemma SN_K_Union:
+  forall K,
+  forall M N, SN (plug K M) -> SN (plug K N) -> SN (plug K (TmUnion M N)).
+Proof.
+ intros K'.
+ pattern K'.
+ apply Ksize_induction_strong; intros.
+
+ clear K'.
+
+ assert (SN M) by (eauto using SN_push_under_k).
+ assert (SN N) by (eauto using SN_push_under_k).
+ assert (Krw_norm K) by (eauto using Krw_norm_from_SN).
+ apply triple_induction_scoped with (K0 := K) (M0 := M) (N0 := N); auto.
+ intros.
+
+ apply reducts_SN.
+ intros Z H_rw.
+
+ destruct K0.
+ - simpl in *.
+   inversion H_rw; subst; auto.
+
+ - simpl in H_rw.
+
+   apply three_ways_to_reduce_at_interface in H_rw as
+       [[[[M' Z_def rw] | [K' Z_def rw]] | [H' [K' [M' ? [? ? H_bogus]]]]] | ?].
+   * (* Case: rw is within TmBind (TmUnion M N) t *)
+     subst.
+     inversion rw; subst.
+     -- (* Case: rw is zippering TmUnion thru TmBind _ _ *)
+       assert (Ksize K0 < Ksize K).
+       { assert (Ksize (Iterate t K0) <= Ksize K).
+         { apply Krw_rt_conserves_Ksize with (K := K); auto. }
+         simpl in *; omega. }
+       apply H; auto.
+       eapply plug_SN_rw_rt with (TmBind M t); auto.
+       { auto using Rw_rt_Bind_left. }
+       change (SN (plug (Iterate t K0) M)).
+       { eauto using SN_via_Krw_rt. }
+       eapply plug_SN_rw_rt with (TmBind N t); auto.
+       { auto using Rw_rt_Bind_left. }
+       change (SN (plug (Iterate t K0) N)).
+       { eauto using SN_via_Krw_rt. }
+     -- (* Case: rw is within TmUnion _ _ *)
+       inversion H14; subst; seauto.
+
+   (* Case: rw is within t of TmBind (TmUnion M N) t *)
+     -- change (SN (plug (Iterate n' K0) (TmUnion M0 N0))).
+        assert (Krw (Iterate t K0) (Iterate n' K0)).
+        ** unfold Krw.
+           simpl.
+           intros.
+           apply Rw_under_K.
+           eauto.
+        ** apply H8.
+           sauto.
+
+   (* Case: rw is within K *)
+   * subst.
+     change (SN (plug (Iterate t K') (TmUnion M0 N0))).
+     apply H8; auto.
+   * (* Case: M is not a bind but it consumes a K frame. *)
+     refute.
+     unfold not in *; eauto using H_bogus.
+     apply NotBind_TmBind in H_bogus; auto.
+   * (* Case: M is a TmBind and we assoc with the context. *)
+     destruct s as [L [L' ? [K' [N' Ha Hb]]]].
+     inversion e.
+     subst.
+     rewrite reverse_plug_defn.
+     apply H.
+     simpl.
+     apply Krw_rt_conserves_Ksize in H5.
+     simpl in *.
+     omega.
+     -- apply SN_via_Krw with (Iterate L' (Iterate N' K')).
+        { apply assoc_in_K. }
+        apply SN_via_Krw_rt with K.
+        auto.
+        apply Rw_trans_preserves_SN with (plug K M).
+        { auto. }
+        { apply Rw_rt_under_K; auto. }
+     -- apply SN_via_Krw with (Iterate L' (Iterate N' K')).
+        { apply assoc_in_K. }
+        apply SN_via_Krw_rt with K.
+        auto.
+        apply Rw_trans_preserves_SN with (plug K N).
+        { auto. }
+        { apply Rw_rt_under_K; auto. }
+Qed.
