Makefile
@@ -23,8 +23,10 @@ OutsideRange.vo: eztactics.v
 
 Continuation.vo: Term.vo Norm.vo
 
+Knorm.vo: Continuation.vo Rewrites.vo Norm.vo Term.vo
+
 sn.vo: eztactics.v Listkit/listkit.vo Term.vo Shift.vo Subst.vo Rewrites.vo \
-	Norm.vo Typing.vo Monomorphism.vo OutsideRange.vo Continuation.vo
+	Norm.vo Typing.vo Monomorphism.vo OutsideRange.vo Continuation.vo Knorm.vo
 
 %.html: %.v %.vo
 	coqdoc -g -d docs $<
@@ -36,17 +38,17 @@ sn.vo: eztactics.v Listkit/listkit.vo Term.vo Shift.vo Subst.vo Rewrites.vo \
 LISTKIT_FILES = Listkit/logickit.v Listkit/NthError.v			\
                 Listkit/Concat.v Listkit/Foreach.v Listkit/Max.v	\
                 Listkit/TakeDrop.v Listkit/RangeSet.v Listkit/All.v	\
-                Listkit/AllType.v Listkit/Map.v Listkit/Sets.v		\
-                Listkit/Subseteq.v
+                Listkit/AllType.v Listkit/Map.v Listkit/Sets.v
 
 Listkit/listkit.vo:
 	make -f Listkit/Makefile $@
 
-FILES = Term.v Shift.v Subst.v Rewrites.v \
+FILES = sn.v Term.v Shift.v Subst.v Rewrites.v Knorm.v \
 	Norm.v Typing.v Monomorphism.v OutsideRange.v Continuation.v \
 	$(LISTKIT_FILES)
 
-index.html: Listkit/listkit.v Term.v Shift.v Subst.v Rewrites.v \
-	Norm.v Typing.v Monomorphism.v OutsideRange.v Continuation.v
+index.html: $(FILES) coqdoc.css
 	mkdir -p docs
-	coqdoc -g --utf8 -d docs $(FILES)
+	coqdoc -g --utf8 -d docs/ $(FILES)
+	# Overwrite the bad CSS coqdoc gives us.
+	cp coqdoc.css docs/
